[CS477][Unit Project] Update invariants for BFS

Formal_Devel_Methods/UnitProject/src/search.dfy
@@ -17,32 +17,6 @@ iterator Iter<T>(S: set<T>) yields (x: T)
   }
 }
 
-/// <summary>
-/// 
-/// </summary>
-class WorkListTrait<T>
-{
-  var tmp : T;
-
-  constructor () {}
-
-  method Enqueue(value: T)
-    modifies this
-  {}
-
-  method Dequeue() returns (value: T)
-    modifies this
-  {
-    return tmp;
-  }
-
-  predicate method empty()
-  {
-    // TODO
-    false
-  }
-}
-
 datatype EdgeBase<T(==)> = EdgeBase(src: T, tgt: T)
 datatype DiGraphBase<T(==)> = DiGraphBase(V: set<T>, E: set<EdgeBase<T>>)
 ///<summary>
@@ -51,20 +25,65 @@ datatype DiGraphBase<T(==)> = DiGraphBase(V: set<T>, E: set<EdgeBase<T>>)
 ///</summary>
 predicate Valid<T(==)>(G: DiGraphBase<T>)
 {
-  forall e :: e in G.E
-     ==> e.src in G.V && e.tgt in G.V
+  (forall e :: e in G.E
+     ==> e.src in G.V && e.tgt in G.V) && (|G.V|>=1)
+}
+///<summary>
+///  Check if every node in the sequence is distinct
+///</summary>
+predicate Unique<T(==)>(list : seq<T>)
+{
+  forall i :: 0 <= i < |list| ==>
+    forall j :: 0 <= j < |list| ==> list[i] == list[j] ==> i == j
+}
+///<summary>
+///  Check if 'path' is a simple path on 'G'
+///</summary>
+predicate ValidSimplePath<T(==)>(G: DiGraphBase<T>, path: seq<T>)
+  requires Valid(G)
+  decreases |path|
+{
+  |path| >= 1 && Unique(path)
+  && forall v :: v in path ==> v in G.V
+  && (|path| > 1 ==>
+     exists e :: e in G.E && e.src == path[|path|-2] && e.tgt == path[|path|-1]
+              && ValidSimplePath(G, path[..(|path|-1)]))
+}
+///<summary>
+///  Check if 's' can reach 't' via path 'p' on 'G'
+///</summary>
+predicate Reachable<T(==)>(G: DiGraphBase<T>, s: T, t:T, p: seq<T>)
+  requires Valid(G)
+{
+  |p| > 0 && p[0] == s && p[|p|-1] == t
+  && ValidSimplePath(G, p) 
 }
 
 datatype NodeT = NIL | NodeT(nat)
 datatype DistT = INF | DistT(l: int)
 datatype Color = WHITE | GREY | BLACK
-datatype NodeLabel = NodeLabel(color: Color, d: DistT, pred: NodeT)
+datatype NodeLabel = NodeLabel(color: Color, d: DistT, ghost pred:seq<NodeT>)
 
 /// <summary>
 /// </summary>
 class SearchAlgorithmBase
 {
   var labels : map<NodeT, NodeLabel>;
+
+  predicate ValidLabels(G : DiGraphBase<NodeT>)
+    reads `labels
+  {
+    forall v :: v in G.V ==> v in labels
+  }
+  predicate InitializedLabels(G : DiGraphBase<NodeT>)
+    reads `labels
+    requires ValidLabels(G)
+  {
+    forall v :: v in G.V
+       ==> (labels[v].color == WHITE
+         && labels[v].d == INF
+         && labels[v].pred == [])
+  }
 
   ///<summary>
   ///</summary>
@@ -82,8 +101,7 @@ class SearchAlgorithmBase
   ///</summary>
   method Init(G: DiGraphBase<NodeT>)
     modifies this;
-    ensures forall v :: v in G.V ==>
-            v in labels && labels[v].color == WHITE;
+    ensures ValidLabels(G) && InitializedLabels(G); 
   {
     var it := new Iter(G.V);
     ghost var X := {};
@@ -94,7 +112,8 @@ class SearchAlgorithmBase
       decreases it.S - X;
       // Custom
       invariant forall v :: v in X
-                ==> v in labels && labels[v].color == WHITE;
+            ==> (v in labels && labels[v].color == WHITE
+                 && labels[v].d == INF && labels[v].pred == []);
     {
       // Iterator code
       var more := it.MoveNext();
@@ -103,8 +122,9 @@ class SearchAlgorithmBase
 
       // Custom code
       var u := it.x;
-      labels := labels[u := NodeLabel(WHITE, INF, NIL)];
+      labels := labels[u := NodeLabel(WHITE, INF, [])];
     }
+    assert X == G.V;
   }
 /* Another version follows for-loop structure
   {
@@ -130,37 +150,88 @@ class SearchAlgorithmBase
   method Search(G: DiGraphBase<NodeT>, s : NodeT)
     modifies this;
     requires Valid(G) && s in G.V;
-    requires forall v :: v in G.V ==>
-             v in labels && labels[v].color == WHITE;
+    requires ValidLabels(G) && InitializedLabels(G); 
+    ensures  ValidLabels(G) 
+    ensures  forall v :: v in G.V && labels[v].color == BLACK
+         ==> labels[v].d != INF && Reachable(G, s, v, labels[v].pred);
   {
     var s_label := labels[s];
-    s_label := s_label.(color := GREY, d := DistT(0));
+    s_label := s_label.(color := GREY, d := DistT(0), pred := [s]);
     labels := labels[s := s_label];
-/*
-    var worklist := new WorkListTrait<NodeT>();
-    worklist.Enqueue(s);
-    ghost var black : set<NodeT> := {};
-    while ( !worklist.empty() )
-      invariant true;
-      decreases G.V - black;
-*/
-    if(true)
+
+    var worklist : seq<NodeT> := [s];
+
+    ghost var B := {};
+    while |worklist| > 0
+      // Aux_LIs_0
+      invariant ValidLabels(G);
+      invariant B == set v | v in G.V && labels[v].color == BLACK;
+      // LI_1
+      invariant forall v :: v in worklist ==> v in G.V;
+      // LI_2 depends on Aux_LIs_0, LI_1
+      invariant forall v :: v in worklist ==> labels[v].color != WHITE;
+      // LI_3 depends on LI_2
+      invariant Unique<NodeT>(worklist);
+      // LI_4 depends on LI_3
+      invariant forall v :: v in worklist ==> labels[v].color != BLACK;
+      // LI_5 depends on Aux LIs, LI_1
+      invariant forall v :: v in worklist ==> labels[v].d != INF;
+      // Termination depends on LI_3, LI_4, Aux_LIs_0
+      decreases G.V - B;
+      // LI_7
+      invariant forall v,n :: v in G.V && n in G.V && labels[v].color == WHITE
+                          ==> v !in labels[n].pred
+      // LI_8 depends on LI_7
+      invariant forall v :: v in worklist
+                        ==> Reachable(G, s, v, labels[v].pred);
+      // LI_9
+      invariant forall v :: v in B
+            ==> labels[v].d != INF && Reachable(G, s, v, labels[v].pred);
     {
-//      var u := worklist.Dequeue();
-      var u := s;
+      // Dequeue
+      var u := worklist[0];
+      worklist := worklist[1..];
+
+      // Color node u to black
+      labels := labels[u := labels[u].(color := BLACK)];
+      B := B + {u};
 
       // Iterate through all outgoing edges of node u
       var edge_u := set e | e in G.E && e.src == u;
       var it := new Iter(edge_u);
       ghost var X := {};
+      ghost var old_labels := labels;
       while(true)
         // Iterator Invariants
         invariant it.Valid() && fresh(it._new);
         invariant X == set z | z in it.xs;
         decreases it.S - X;
         // Custom Invariants
-        invariant forall v :: v in G.V ==> v in labels;
-        invariant labels[u].d != INF;
+        // Aux_LIs_0
+        invariant ValidLabels(G) && forall v :: v in G.V ==> v in old_labels;
+        invariant B == set v | v in G.V && labels[v].color == BLACK;
+        // LI_1
+        invariant forall v :: v in worklist ==> v in G.V;
+        // LI_2 depends on Aux_LIs_0, LI_1
+        invariant forall v :: v in worklist ==> labels[v].color != WHITE;
+        // LI_3 depends on LI_2
+        invariant Unique<NodeT>(worklist);
+        // LI_4 depends on LI_3
+        invariant forall v :: v in worklist ==> labels[v].color != BLACK;
+        // LI_5 depends on Aux_LIs_0, LI_1
+        invariant forall v :: v in worklist ==> labels[v].d != INF;
+        // LI_6 depends on LI_5
+        invariant u in labels && labels[u].d != INF;
+        // LI_7
+        invariant forall v,n :: v in G.V && n in G.V && labels[v].color == WHITE
+              ==> v !in labels[n].pred
+        // LI_8 depends on LI_7
+        invariant Reachable(G, s, u, labels[u].pred)
+               && forall v :: v in worklist
+                          ==> Reachable(G, s, v, labels[v].pred)
+        // LI_9
+        invariant forall v :: v in B 
+              ==> labels[v].d != INF && Reachable(G, s, v, labels[v].pred);
       {
         // Iterator Code
         var more := it.MoveNext();
@@ -168,23 +239,22 @@ class SearchAlgorithmBase
         X := X + {it.x};
 
         // Custom Code
-        var v := it.x.tgt;
+        var v : NodeT := it.x.tgt;
         if(labels[v].color == WHITE)
         {
           var v_label := labels[v];
-          assert labels[u].d != INF;
+          assert labels[u].d != INF; // Proven by LI_6
           v_label := v_label.(
             color := GREY,
             d := DistT(labels[u].d.l + 1),
-            pred := u
+            pred := labels[u].pred + [v]
           );
+          assert Reachable(G, s, v, v_label.pred); // Proven by LI_7. Help prove LI_8
           labels := labels[v := v_label];
-          //worklist.Enqueue(v);
+          // Enqueue
+          worklist := worklist + [v];
         }
       }
-      // Color node u to black
-      labels := labels[u := labels[u].(color := BLACK)];
-//      black := black + {u};
     }
   }
 }
